progs/verif_message.v
@@ -119,7 +119,7 @@ simpl.
 rewrite sepcon_comm.
 apply sepcon_derives; apply derives_refl';
  eapply mapsto_field_mapsto; unfold field_offset; try (simpl; reflexivity);
-destruct buf0; inv H0; reflexivity.
+destruct buf0; inv H0; unfold eval_binop; simpl; f_equal; rewrite Int.add_assoc; f_equal.
 Qed.
 
 Lemma body_intpair_deserialize: semax_body Vprog Gtot f_intpair_deserialize intpair_deserialize_spec.
@@ -147,7 +147,9 @@ apply semax_pre_PQR with
         (`(add_ptr_int tint) (`(eval_cast (tptr tuchar) (tptr tint)) (eval_id _buf)) `1)
         `(Vint y1))).
 go_lower; subst. unfold intpair_message.
- simpl_typed_mapsto.  rewrite (field_mapsto_isptr). normalize. 
+ simpl_typed_mapsto.  simpl. rewrite (field_mapsto_isptr). normalize.
+ repeat apply andp_right; try apply prop_right; auto.
+ destruct buf0; inv H0; auto.
  cancel.
 apply sepcon_derives; apply derives_refl'';
  eapply mapsto_field_mapsto; unfold field_offset; try (simpl; reflexivity);
@@ -167,89 +169,17 @@ cancel.
 simpl. rewrite sepcon_comm.
 apply sepcon_derives;
 apply derives_refl'; eapply mapsto_field_mapsto;  unfold field_offset; try (simpl; reflexivity);
- destruct buf0; inv H0; reflexivity.
+ destruct buf0; inv H0; unfold eval_binop; simpl; reflexivity.
 Qed.
 
-
-Ltac start_function := 
- match goal with |- semax_body _ _ _ ?spec => try unfold spec end;
- match goal with |- semax_body _ _ _ (pair _ (mk_funspec _ _ ?Pre _)) =>
-   match Pre with 
-   | (fun x => match x with (a,b) => _ end) => intros [a b] 
-   | (fun i => _) => intro i
-   end;
-   simpl fn_body; simpl fn_params; simpl fn_return
- end;
- repeat match goal with |- semax _ (match ?p with (a,b) => _ end * _) _ _ =>
-             destruct p as [a b]
-           end;
- match goal with |- semax (func_tycontext ?F ?V ?G) _ _ _ => 
-   set (Delta := func_tycontext F V G)
- end;
-  match goal with
-  | |- semax _ (?P * stackframe_of ?F) _ _ =>
-            change (stackframe_of F) with (@emp assert _ _);
-            rewrite sepcon_emp;
-            rewrite frame_ret_assert_emp
-  | |- semax _ ((PROPx ?P (LOCALx ?Q (SEPx ?R))) * stackframe_of ?F) _ _ =>
-        change (@LiftNatDed environ mpred Nveric) with Nassert;
-        change (@LiftSepLog environ mpred Nveric Sveric) with Sassert;
-        rewrite (start_function_aux1 (stackframe_of F) P Q R)
- | |- _ => idtac
-  end;
- match goal with
-  | |- semax _ (PROPx _ _) _ _ => idtac 
-  | _ => canonicalize_pre 
- end;
- repeat (apply semax_extract_PROP; intro).
-
-
-Lemma memory_block_isptr: forall sh i v, 
-  i > 0 -> 
-  memory_block sh (Int.repr i) v = !!(isptr v) && memory_block sh (Int.repr i) v.
-Proof.
-Admitted.  (* not difficult *)
-
-Lemma typed_mapsto__isptr:
-  forall sh t v, typed_mapsto_ sh t v = !!(isptr v) && typed_mapsto_ sh t v.
-Proof.
-intros.
-rewrite <- memory_block_typed.
-apply memory_block_isptr.
-apply sizeof_pos.
-Qed.
-
-Lemma var_block_typed_mapsto_:
-  forall  sh id t, 
- var_block sh (id, t) = `(typed_mapsto_ (Share.splice sh Share.top) t) (eval_var id t).
-Proof.
-intros; extensionality rho.
-unfold_coerce.
-rewrite <- memory_block_typed.
-unfold var_block, lvalue_block.
-rewrite memory_block_isptr by apply sizeof_pos.
-simpl.
-destruct (eval_var id t rho); simpl; normalize.
-Admitted.
-
-
-Lemma var_block_typed_mapsto__top:
-  forall id t, 
- var_block Share.top (id, t) = `(typed_mapsto_ Share.top t) (eval_var id t).
-Proof.
-intros.
-rewrite var_block_typed_mapsto_.
-rewrite splice_top_top; auto.
-Qed.
+Ltac simpl_stackframe_of := 
+  unfold stackframe_of, fn_vars; simpl map; unfold fold_right; rewrite sepcon_emp;
+  repeat rewrite var_block_typed_mapsto__top. 
 
 Lemma body_main:  semax_body Vprog Gtot f_main main_spec.
 Proof.
-start_function.
-unfold stackframe_of, fn_vars. simpl map. unfold fold_right.
-repeat rewrite var_block_typed_mapsto__top.
-
-
-
+start_function. simpl_stackframe_of.
+repeat simpl_typed_mapsto.
 
 
 
